A,B,C 均是M的子集
1.1 $(A\subset C )\wedge (B \subset C )\iff (A\cup B)\subset C$
$(\implies)$ $x\in A \cup B\iff x\in A \vee x\in B\implies x\in C\vee x\in C\implies x\in C$
$(\impliedby)$ $A\subset A\cup B\subset C. B\subset A\cup B\subset C\implies A\subset C \wedge B\subset C$
1.2$(C\subset A)\wedge (C\subset B)\iff (C\subset A\cap B)$
$(\implies)(x\in C\implies x \in A) \wedge (x\in C\implies x\in B)\implies x\in A\cap B$$(\impliedby)x\in C\implies x\in A\wedge x\in B\implies (x\in C \implies x\in A )\wedge (x\in C\implies x\in B)\iff (C\subset A)\wedge(C\subset B)$
1.3 $C_M(C_M A)=A$
$C_M(C_M A)=M\backslash(M\backslash A)=M\cap A=A$
$(R\backslash(S\backslash T)=(R\backslash T)\cup(R\cap T))$
$(T\subset S\iff T\cap S=T$）

1.4
$A\subset C_M B\iff B\subset C_M A$
$A\subset C_M B\iff A\cap C_M B=A\iff A\cap M\backslash B=A\iff A\cap M-A\cap B=A$$\iff A-A\cap B=A\iff A\cap B=\emptyset$
$B\subset C_M A\iff B\cap C_M A=B\iff B\cap M\backslash A=B\iff B\cap M-A\cap B=B$
$\iff B-A\cap B=B\iff A\cap B=\emptyset$

因此$LHS\iff RHS$
1.5$A\subset B$$\iff$$C_M A\supset C_M B$
$A\subset B\iff A\cap B=A\iff$
$C_M A\cap C_M B=C_M B\iff M\backslash A\cap M \backslash B=M\backslash B\iff M\backslash (A\cup B)=M\backslash B\iff A\subset B$

2.1
$x\in (A\cup B) \cup C\iff x\in A \vee x\in B\vee x\in C$
$x\in A\cup (B \cup C)$$\iff x\in A\vee x\in B\vee x\in C$
$x\in A\cup B \cup C \iff x\in A\vee x\in B\vee x\in C$
$\implies$ $(A\cup B)\cup C=A\cup(B\cup C)=A\cup B\cup C$

2.2
$x\in A\cap (B\cap C)\iff x\in A\wedge x\in B \wedge x\in C$
$x\in (A\cap B)\cap C\iff x\in A\wedge x\in B\wedge x\in C$
$x\in A\cap B\cap C\iff x\in A\wedge x\in B\wedge x\in C$
$\implies A\cap(B\cap C)=(A\cap B)\cap C=A\cap B\cap C$

2.3
$A\cap (B\cup C)=(A\cap B)\cup(A\cap C)$
$(\implies)x\in A\cap(B\cup C)\implies$ x 属于A 和 (x 属于B 或 x 属于 C)
If $x\in B$, $x\in A\cap B$, if $x\in C$,$x\in A\cap C$ 
因为 $x \in B\cup C$ ，我们有 $x\in (A\cap B) \cup (A\cap C)$
$\implies A\cap (B\cup C)\subset (A\cap B)\cup(A\cap C)$
$(\impliedby)x\in (A\cap B)\cup(A\cap C)\implies x\in A\cap B$ or  $x\in A\cap C$
我们总是有$x\in A$ 且$A\cap B\subset B\subset B\cup C$,且$A\cap C\subset C\subset B\cup C$
所以 $x\in A\cap (B\cup C)$
$\implies A\cap (B\cup C)\supset (A\cap B)\cup(A\cap C)$
于是 $A\cap (B\cup C)=(A\cap B)\cup(A\cap C)$

2.4
$A\cup (B\cap C)=(A\cup B)\cap(A\cup C)$
$(\implies)x\in A\cup(B\cap C)\implies x\in A$ or $x\in B\cap C$
若$x\in A,A\subset A\cup B,A\subset A\cup C$故$x\in A\implies (A\cup B)\cap(A\cup C)$
若$x\in B\cap C,B\cap C\subset B\subset A\cup B,B\cap C\subset C\subset A\cup C$
故$x\in B\cap C\implies x\in (A\cup B)\cap(A\cup C)$
于是，$x\in A\cup (B\cap C)\implies x\in (A\cup B)\cap(A\cup C)$
$(\impliedby)x\in (A\cup B)\cap (A\cup C)$
若$x\in A$，$A\subset A\cup (B\cap C)$则$x\in A\cup(B\cap C)$
若$x\notin A$则$x\in B\cap C$(因为$x\in A\cup B$且$x\in A\cup C$)
于是不管是哪个情况，我们都有$x\in A\cup (B\cap C)$
故$A\cup (B\cap C)=(A\cup B)\cap(A\cup C)$

3.1
$C_M(A\cup B)=C_M A \cap C_M B$
$x\in C_M(A\cup B)\iff x\in M\wedge \neg(x\in A\cup B)\iff x\in M\wedge x\notin A\wedge x\notin B$
$x\in C_M A\cap C_M B\iff x\in C_M A\wedge x\in C_M B\iff x\in M\wedge x\notin A\wedge x\notin B$
$\therefore LHS\iff RHS$
3.2
$C_M(A\cap B)=C_M A\cup C_M B$
$x\in C_M(A\cap B)\iff x\in M\wedge \neg(x\in A\cap B)\iff x\in M\wedge(x\notin A\vee x\notin B)$
$x\in C_M A\cup C_M B\iff (x\in M\wedge x\notin A)\vee(x\in M\wedge x\notin B)\iff x\in M\wedge(x\notin A\vee x\notin B)$
$\therefore LHS\iff RHS$

